compiler/src/compiler/util/Result.v
@@ -1,0 +1,161 @@
+(* Almost everyone importing this file will need strings in their error messages *)
+Require Export Coq.Strings.String. Open Scope string_scope.
+
+Inductive dlist: Type :=
+| dnil
+| dcons{T: Type}(head: T)(tail: dlist).
+
+Inductive result{A: Type}: Type :=
+| Success(a: A)
+| Failure(msg: dlist).
+Arguments result: clear implicits.
+
+Declare Scope error_scope.
+Open Scope error_scope.
+
+Notation "'error:(' x )" := (Failure (dcons x dnil))
+  (at level 0, x at level 0, format "'error:(' x )")
+  : error_scope.
+
+Notation "'error:(' x y .. z )" := (Failure (dcons x (dcons y .. (dcons z dnil) ..)))
+  (at level 0, x at level 0, y at level 0, z at level 0, format "'error:(' x  y  ..  z )")
+  : error_scope.
+
+Goal @id (result nat) error:(4 "is not a" bool) =
+     Failure (dcons 4 (dcons "is not a" (dcons bool dnil))).
+Proof. reflexivity. Abort.
+
+Goal error:("just one string") = @Failure nat (dcons "just one string" dnil).
+Proof. reflexivity. Abort.
+
+Goal (fun (x: option nat) =>
+        match x with
+        | Some v => Success v
+        | None => error:("got" x "instead of" (@Some nat))
+        end) None <> Success 0.
+Proof. cbv. congruence. Abort.
+
+(* Note: won't parse if we remove the space after the colon *)
+Goal forall (error: (list nat)), nil = (error: (list nat)). Abort.
+
+Module result.
+  Definition of_option{A: Type}(o: option A): result A :=
+    match o with
+    | Some a => Success a
+    | None => error:((option A) "was" o)
+    end.
+End result.
+
+Module ResultMonadNotations.
+  Declare Scope result_monad_scope.
+  Open Scope result_monad_scope.
+
+  Notation "' pat <- c1 ;; c2" :=
+    (match c1 with
+     | Success pat => c2
+     | Failure e => Failure e
+     end)
+    (at level 60, pat pattern, c1 at next level, right associativity) : result_monad_scope.
+
+  Notation "x <- c1 ;; c2" :=
+    (match c1 with
+     | Success x => c2
+     | Failure e => Failure e
+     end)
+    (at level 60, c1 at next level, right associativity) : result_monad_scope.
+
+  Notation "c1 ;; c2" :=
+    (match c1 with
+     | Success _ => c2
+     | Failure e => Failure e
+     end)
+    (at level 60, right associativity) : result_monad_scope.
+End ResultMonadNotations.
+
+Module List.
+  Import ResultMonadNotations.
+  Section WithA.
+    Context {A: Type}.
+
+    Fixpoint all_success(rs : list (result A)): result (list A) :=
+      match rs with
+      | nil => Success nil
+      | cons r rest => x <- r;; xs <- all_success rest;; Success (cons x xs)
+      end.
+
+    Lemma length_all_success: forall {l1: list (result A)} {l2: list A},
+        all_success l1 = Success l2 ->
+        List.length l2 = List.length l1.
+    Proof.
+      induction l1; cbn; intros.
+      { inversion H. trivial. }
+      { case a in *; try inversion H.
+        case (all_success l1) in *; try inversion H.
+        subst. cbn. eapply f_equal, IHl1; trivial. }
+    Qed.
+  End WithA.
+End List.
+
+Require Import coqutil.Map.Interface coqutil.Map.Properties.
+Require Import coqutil.Decidable.
+Require Import coqutil.Tactics.fwd.
+Require Import coqutil.Tactics.destr.
+
+Module map.
+  Import ResultMonadNotations.
+
+  Section WithMap.
+    Context {key value : Type} {map : map.map key value} {map_ok : map.ok map}
+            {keqb: key -> key -> bool} {keqb_spec: EqDecider keqb}.
+
+    Definition forall_success(f: key -> value -> result unit): map -> result unit :=
+      map.fold (fun res k v => res;; f k v) (Success tt).
+
+    Lemma get_forall_success: forall f m,
+        forall_success f m = Success tt -> forall k v, map.get m k = Some v -> f k v = Success tt.
+    Proof.
+      unfold forall_success. intros f m.
+      eapply map.fold_spec; intros.
+      - rewrite map.get_empty in H0. discriminate.
+      - fwd. rewrite map.get_put_dec in H2. destr (keqb k k0); fwd; eauto.
+    Qed.
+  End WithMap.
+
+  Section WithTwoMaps.
+    Context {K V1 V2: Type}{M1: map.map K V1}{M2: map.map K V2}
+            {keqb: K -> K -> bool} {keqb_spec: EqDecider keqb}
+            {OK1: map.ok M1} {OK2: map.ok M2}.
+
+    Definition try_map_values(f: V1 -> result V2): M1 -> result M2 :=
+      map.fold (fun acc_res k v1 => acc <- acc_res;; v2 <- f v1;; Success (map.put acc k v2))
+               (Success map.empty).
+
+    Lemma try_map_values_fw(f: V1 -> result V2)(m1: M1)(m2: M2):
+        try_map_values f m1 = Success m2 ->
+        forall (k: K) (v1: V1),
+        map.get m1 k = Some v1 ->
+        exists v2, f v1 = Success v2 /\ map.get m2 k = Some v2.
+    Proof.
+      unfold try_map_values. revert m2.
+      eapply map.fold_spec; intros.
+      - rewrite map.get_empty in H0. discriminate.
+      - fwd.
+        rewrite map.get_put_dec. rewrite map.get_put_dec in H2.
+        destr (keqb k k0); fwd; eauto.
+    Qed.
+
+    Lemma try_map_values_bw(f: V1 -> result V2)(m1: M1)(m2: M2):
+        try_map_values f m1 = Success m2 ->
+        forall (k: K) (v2: V2),
+        map.get m2 k = Some v2 ->
+        exists v1, f v1 = Success v2 /\ map.get m1 k = Some v1.
+    Proof.
+      unfold try_map_values. revert m2.
+      eapply map.fold_spec; intros.
+      - fwd. rewrite map.get_empty in H0. discriminate.
+      - fwd.
+        rewrite map.get_put_dec. rewrite map.get_put_dec in H2.
+        destr (keqb k k0); fwd; eauto.
+    Qed.
+  End WithTwoMaps.
+End map.
